change monad in block

Freigen/Circuit/Defs.lean
@@ -4,47 +4,98 @@ import Freigen.Free
 
 namespace Freigen.Circuit
 
-inductive Eff : Type _
-| assert
-| hint (tp : Type)
+inductive Scope : Type u where
+| constraint
+| hint
 
-def Eff.input : Eff → Type _
-| .assert => Bool
-| .hint _ => Unit
+inductive ConstraintEff where
+| assert_r1c
+| rangecheck (n: Nat)
+| assert_spread (n: Nat)
+| one
+| hint (n : Nat) (α : Type)
 
-def Eff.output : Eff → Type
-| .assert => Unit
-| .hint tp => tp
+inductive HintEff : Type u where
+| write_witness
 
-def Eff.blockTag : Eff → Type _
-| .assert => PEmpty
-| .hint _ => PUnit
+def Eff (W F : Type) : Scope → Type _
+| .constraint => ConstraintEff
+| .hint => HintEff
 
-def Eff.blockInputs : (t : Eff) → Eff.blockTag t → Type
-| assert => nofun
-| hint _ => fun _ => Unit
-
-def Eff.blockOutputs : (t : Eff) → Eff.blockTag t → Type
-| assert => nofun
-| hint tp => fun _ => tp
-
-instance : Freigen.Eff.Spec Eff where
-  input := Eff.input
-  output := Eff.output
-  blockTag := Eff.blockTag
-  blockInputs := Eff.blockInputs
-  blockOutputs := Eff.blockOutputs
+instance {W F} : Freigen.Eff.Spec (Γ := Scope) (Eff W F) where
+  input := fun
+  | .constraint, .assert_r1c => W × W × W
+  | .constraint, .rangecheck _ => W
+  | .constraint, .assert_spread _ => W × W
+  | .constraint, .one => Unit
+  | .constraint, .hint n _ => Vector W n
+  | .hint, .write_witness => F
+  output := fun
+  | .constraint, .assert_r1c => Unit
+  | .constraint, .rangecheck _ => Unit
+  | .constraint, .assert_spread _ => Unit
+  | .constraint, .one => W
+  | .constraint, .hint _ α => α
+  | .hint, .write_witness => W
+  blockTag := fun
+  | .constraint, .assert_r1c => PEmpty
+  | .constraint, .rangecheck _ => PEmpty
+  | .constraint, .assert_spread _ => PEmpty
+  | .constraint, .one => PEmpty
+  | .constraint, .hint _ _ => PUnit
+  | .hint, .write_witness => PEmpty
+  blockCtx := fun
+  | .constraint, .assert_r1c => nofun
+  | .constraint, .rangecheck _ => nofun
+  | .constraint, .assert_spread _ => nofun
+  | .constraint, .one => nofun
+  | .constraint, .hint _ _ => fun _ => .hint
+  | .hint, .write_witness => nofun
+  blockInputs := fun
+  | .constraint, .assert_r1c => nofun
+  | .constraint, .rangecheck _ => nofun
+  | .constraint, .assert_spread _ => nofun
+  | .constraint, .one => nofun
+  | .constraint, .hint n _ => fun _ => Vector F n
+  | .hint, .write_witness => nofun
+  blockOutputs := fun
+  | .constraint, .assert_r1c => nofun
+  | .constraint, .rangecheck _ => nofun
+  | .constraint, .assert_spread _ => nofun
+  | .constraint, .one => nofun
+  | .constraint, .hint _ α => fun _ => α
+  | .hint, .write_witness => nofun
 
 end Circuit
 
-def Circuit : Type → Type _ := Free Circuit.Eff
+def Circuit (F : Type) (W : Type) : Type → Type _ := Free (Circuit.Eff W F) .constraint
+
+instance {F W} : Monad (Circuit F W) := inferInstanceAs (Monad (Free (Circuit.Eff W F) .constraint))
+instance {F W} : LawfulMonad (Circuit F W) := inferInstanceAs (LawfulMonad (Free (Circuit.Eff W F) .constraint))
 
 namespace Circuit
 
-def assert (b : Bool) : Circuit Unit :=
-  Free.op (E := Circuit.Eff) Eff.assert b nofun
+def Hint (F : Type) (W : Type) : Type → Type _ := Free (Circuit.Eff W F) .hint
 
-def hint {α : Type} : Circuit α → Circuit α := fun hint =>
-  Free.op (E := Circuit.Eff) (Eff.hint α) () fun _ _ => hint
+instance {F W} : Monad (Hint F W) := inferInstanceAs (Monad (Free (Circuit.Eff W F) .hint))
+instance {F W} : LawfulMonad (Hint F W) := inferInstanceAs (LawfulMonad (Free (Circuit.Eff W F) .hint))
+
+def assert_r1c {F W} (a b c : W) : Circuit F W Unit :=
+  Free.op (E := Circuit.Eff W F) (γ := .constraint) .assert_r1c (a, b, c) nofun
+
+def rangecheck {F W} (n : Nat) (a : W) : Circuit F W Unit :=
+  Free.op (E := Circuit.Eff W F) (γ := .constraint) (.rangecheck n) a nofun
+
+def assert_spread {F W} (n : Nat) (a b : W) : Circuit F W Unit :=
+  Free.op (E := Circuit.Eff W F) (γ := .constraint) (.assert_spread n) (a, b) nofun
+
+def one {F W} : Circuit F W W :=
+  Free.op (E := Circuit.Eff W F) (γ := .constraint) .one PUnit.unit nofun
+
+def hint {F W α} (n : Nat) (args : Vector W n) (h : Hint F W α) : Circuit F W α :=
+  Free.op (E := Circuit.Eff W F) (γ := .constraint) (.hint n α) args fun _ _ => h
+
+def write_witness {F W} (a : F) : Hint F W W :=
+  Free.op (E := Circuit.Eff W F) (γ := .hint) .write_witness a nofun
 
 end Freigen.Circuit
