Freigen/CompM/Basic.lean
@@ -4,17 +4,26 @@ import Freigen.Eff
 
 namespace Freigen
 
-def CompM (E : Type u) [Eff.Spec E] (α : Type) : Type _ :=
-  ExactCodensity (ITree E) α
+def CompM
+    {Γ : Type u} (E : Γ → Type u) [Eff.Spec E]
+    (γ : Γ) (α : Type v) : Type _ :=
+  ExactCodensity (ITree E γ) α
 
-variable {E : Type u} [eS: Eff.Spec E] {α β : Type}
+variable
+  {Γ : Type u} {E : Γ → Type u} [eS : Eff.Spec E]
+  {γ : Γ} {α β : Type}
 
-instance {E : Type u} [Eff.Spec E] : Monad (CompM E) := inferInstanceAs (Monad (ExactCodensity (ITree E)))
-instance {E : Type u} [Eff.Spec E] : LawfulMonad (CompM E) := inferInstanceAs (LawfulMonad (ExactCodensity (ITree E)))
+instance {γ : Γ} : Monad (CompM E γ) :=
+  inferInstanceAs (Monad (ExactCodensity (ITree E γ)))
+
+instance {γ : Γ} : LawfulMonad (CompM E γ) :=
+  inferInstanceAs (LawfulMonad (ExactCodensity (ITree E γ)))
 
 namespace CompM
 
-private theorem bind_def {α β : Type _} (x : CompM E α) (f : α → CompM E β) :
+private theorem bind_def
+    {γ : Γ} {α β : Type}
+    (x : CompM E γ α) (f : α → CompM E γ β) :
     x >>= f = ⟨fun g => x.run fun a => (f a).run g, by
       intros
       conv => lhs; rw [←x.exact]
@@ -22,15 +31,26 @@ private theorem bind_def {α β : Type _} (x : CompM E α) (f : α → CompM E �
       simp only [ExactCodensity.exact]⟩ := by
   rfl
 
-def tick [Eff.Has Eff.Tau E] : CompM E Unit := ⟨fun f => ITree.tau (f ()), by simp⟩
+def tick {γ : Γ} [Eff.Has.{u, 0} Eff.Tau E] :
+    CompM E γ Unit :=
+  ⟨fun f => ITree.tau (f ()), by simp⟩
 
-def fail [Eff.Has Eff.Fail E] : CompM E α := ⟨fun f => ITree.fail, by simp⟩
+def fail {γ : Γ} [Eff.Has Eff.Fail E] :
+    CompM E γ α :=
+  ⟨fun _ => ITree.fail, by simp⟩
 
-def op (e : E) (inp : eS.input e)
-    (blocks : (t : eS.blockTag e) → eS.blockInputs e t → CompM E (eS.blockOutputs e t)): CompM E (eS.output e) :=
+def op {γ : Γ} (e : E γ) (inp : eS.input γ e)
+    (blocks :
+      (t : eS.blockTag γ e) →
+      eS.blockInputs γ e t →
+      CompM E (eS.blockCtx γ e t) (eS.blockOutputs γ e t)) :
+    CompM E γ (eS.output γ e) :=
   ⟨fun f => ITree.op e inp (fun t i => (blocks t i).run pure) f, by simp⟩
 
-def loop [Eff.Has Eff.Tau E] (body : α → CompM E (α ⊕ β)) (init : α): CompM E β := {
+def loop
+    {γ : Γ} [Eff.Has Eff.Tau E]
+    (body : α → CompM E γ (α ⊕ β)) (init : α) :
+    CompM E γ β := {
   run := fun f => ITree.loop (fun a => (body a).run pure) init f
   exact := by
     intros
@@ -38,17 +58,19 @@ def loop [Eff.Has Eff.Tau E] (body : α → CompM E (α ⊕ β)) (init : α): Co
 }
 
 theorem loop_def [Eff.Has Eff.Tau E]
-  (body : α → CompM E (α ⊕ β))
+  (body : α → CompM E γ (α ⊕ β))
   (s : α) :
   CompM.loop body s =
     body s >>= fun
       | .inr v  => pure v
-      | .inl v => CompM.tick *> CompM.loop body v := by
+      | .inl v => CompM.tick (E := E) (γ := γ) *> CompM.loop body v := by
   apply ExactCodensity.equiv.injective
   change (CompM.loop body s).run pure =
     ((body s >>= fun
       | .inr v => pure v
-      | .inl v => CompM.tick *> CompM.loop body v) : CompM E β).run pure
+      | .inl v =>
+        CompM.tick (E := E) (γ := γ) *> CompM.loop body v) :
+        CompM E γ β).run pure
   simp only [loop, bind_def]
   rw [ITree.loop_def]
   rw [ExactCodensity.exact]
@@ -60,7 +82,8 @@ abbrev forInStepToSum : ForInStep α → α ⊕ α
   | .yield x => .inl x
   | .done x => .inr x
 
-instance [Eff.Has Eff.Tau E] : ForIn (CompM E) Lean.Loop Unit where
+instance {γ : Γ} [Eff.Has Eff.Tau E] :
+    ForIn (CompM E γ) Lean.Loop Unit where
   forIn _ init body := loop (fun a => forInStepToSum <$> (body () a)) init
 
 end Freigen.CompM
