Freigen/Eff.lean
@@ -2,67 +2,90 @@ import Freigen.IxPoly.Basic
 
 namespace Freigen.Eff
 
-class Spec (tag : Type u) where
-  input : tag → Type v
-  output : tag → Type v
-  blockTag : tag → Type u
-  blockInputs : (t : tag) → blockTag t → Type v
-  blockOutputs : (t : tag) → blockTag t → Type v
+class Spec {Γ : Type u} (tag : Γ → Type u) where
+  input : (γ : Γ) → tag γ → Type v
+  output : (γ : Γ) → tag γ → Type v
+  blockTag : (γ : Γ) → tag γ → Type u
+  blockCtx : (γ : Γ) → (t : tag γ) → blockTag γ t → Γ
+  blockInputs : (γ : Γ) → (t : tag γ) → blockTag γ t → Type v
+  blockOutputs : (γ : Γ) → (t : tag γ) → blockTag γ t → Type v
 
-inductive NodeTag (T : Type u) [s: Spec T] : Type _ → Type _ where
-| ret {R} : R → NodeTag T R
-| op {R} (t : T) : s.input t → NodeTag T R
+inductive NodeTag (Γ : Type u) (T : Γ → Type u) [s : Spec.{u, v} T]
+    (γ : Γ) (R : Type v) : Type (max u v) where
+| ret : R → NodeTag Γ T γ R
+| op (t : T γ) : s.input γ t → NodeTag Γ T γ R
 
-def NodeTag.fields {i} {T : Type u} [s : Spec T]: NodeTag T i → Type _
+abbrev NodeTag.fields {Γ : Type u} {T : Γ → Type u} {γ} [s : Spec T]
+    {R : Type v} : NodeTag Γ T γ R → Type (max u v)
 | ret _ => PEmpty
-| op e _ => s.output e ⊕ ((t : s.blockTag e) × s.blockInputs e t)
+| op e _ => s.output γ e ⊕ ((t : s.blockTag γ e) × s.blockInputs γ e t)
 
-def NodeTag.elem {T : Type u} [s : Spec T] {α : Type v} :
-    (t : NodeTag T α) → (p : t.fields) → Type v
-| ret _, x => nomatch x
-| op _ _, Sum.inl _ => α
-| op e _, Sum.inr ⟨o, _⟩ => s.blockOutputs e o
+def NodeTag.elem {Γ : Type u} {T : Γ → Type u} {γ} [s : Spec T] {α : Type v} :
+    (t : NodeTag Γ T γ α) → (p : t.fields) → Γ × Type v
+| ret _ => nofun
+| op e _ => fun
+  | Sum.inl _ => (γ, α)
+  | Sum.inr ⟨o, _⟩ => (s.blockCtx γ e o, s.blockOutputs γ e o)
 
-instance : Spec PEmpty where
+def NoEff {Γ : Type u} : Γ → Type u := fun _ => PEmpty
+
+instance {Γ : Type u} : Spec (@NoEff Γ) where
   input := nofun
   output := nofun
   blockTag := nofun
+  blockCtx := nofun
   blockInputs := nofun
   blockOutputs := nofun
 
-instance sumInst {T₁ T₂ : Type u} [Spec T₁] [Spec T₂] : Spec (T₁ ⊕ T₂) where
-  input := fun
-    | Sum.inl t => Spec.input t
-    | Sum.inr t => Spec.input t
-  output := fun
-    | Sum.inl t => Spec.output t
-    | Sum.inr t => Spec.output t
-  blockTag := fun
-    | Sum.inl t => Spec.blockTag t
-    | Sum.inr t => Spec.blockTag t
-  blockInputs := fun
-    | Sum.inl t => Spec.blockInputs t
-    | Sum.inr t => Spec.blockInputs t
-  blockOutputs := fun
-    | Sum.inl t => Spec.blockOutputs t
-    | Sum.inr t => Spec.blockOutputs t
+def Sum {Γ : Type u} (T₁ T₂ : Γ → Type u) : Γ → Type u := fun γ => T₁ γ ⊕ T₂ γ
 
-class inductive Has : (a: Type u) → [Spec a] → (b: Type u) → [Spec b] → Type _ where
-| here {α : Type u} [s : Spec α] : Has α α
-| inl {α β γ : Type u} [Spec α] [Spec β] [Spec γ] : Has α β → Has α (β ⊕ γ)
-| inr {α β γ : Type u} [Spec α] [Spec β] [Spec γ] : Has α γ → Has α (β ⊕ γ)
+infix:65 " ⊕ₑ " => Sum
+
+instance sumInst {Γ : Type u} {T₁ T₂ : Γ → Type u}
+    [Spec T₁] [Spec T₂] : Spec (T₁ ⊕ₑ T₂) where
+  input := fun
+    | γ, Sum.inl t => Spec.input γ t
+    | γ, Sum.inr t => Spec.input γ t
+  output := fun
+    | γ, Sum.inl t => Spec.output γ t
+    | γ, Sum.inr t => Spec.output γ t
+  blockTag := fun
+    | γ, Sum.inl t => Spec.blockTag γ t
+    | γ, Sum.inr t => Spec.blockTag γ t
+  blockCtx := fun
+    | γ, Sum.inl t, b => Spec.blockCtx γ t b
+    | γ, Sum.inr t, b => Spec.blockCtx γ t b
+  blockInputs := fun
+    | γ, Sum.inl t => Spec.blockInputs γ t
+    | γ, Sum.inr t => Spec.blockInputs γ t
+  blockOutputs := fun
+    | γ, Sum.inl t => Spec.blockOutputs γ t
+    | γ, Sum.inr t => Spec.blockOutputs γ t
+
+class inductive Has {Γ : Type u} :
+    (a : Γ → Type u) → [Spec a] →
+    (b : Γ → Type u) → [Spec b] → Type _ where
+| here {α : Γ → Type u} [s : Spec α] : Has α α
+| inl {α β γ : Γ → Type u}
+    [Spec α] [Spec β] [Spec γ] :
+    Has α β → Has α (β ⊕ₑ γ)
+| inr {α β γ : Γ → Type u}
+    [Spec α] [Spec β] [Spec γ] :
+    Has α γ → Has α (β ⊕ₑ γ)
 
 instance [Spec α] : Has α α := Has.here
-instance [Spec α] [Spec β] [Spec γ] [r: Has α β] : Has α (β ⊕ γ) := Has.inl r
-instance [Spec α] [Spec β] [Spec γ] [r: Has α γ] : Has α (β ⊕ γ) := Has.inr r
+instance [Spec α] [Spec β] [Spec γ] [r : Has α β] :
+    Has α (β ⊕ₑ γ) := Has.inl r
+instance [Spec α] [Spec β] [Spec γ] [r : Has α γ] :
+    Has α (β ⊕ₑ γ) := Has.inr r
 
-def Has.mk {α β} [Spec α] [Spec β] [r: Has α β] : α → β
+def Has.mk {Γ} {α β : Γ → Type u} {γ : Γ} [Spec α] [Spec β] [r: Has α β] : α γ → β γ
 | a => match r with
   | Has.here => a
   | Has.inl r => Sum.inl (Has.mk a)
   | Has.inr r => Sum.inr (Has.mk a)
 
-def Has.out {α β} [Spec α] [Spec β] [r: Has α β] : β → Option α
+def Has.out {Γ} {α β : Γ → Type u} {γ : Γ} [Spec α] [Spec β] [r: Has α β] : β γ → Option (α γ)
 | b => match r, b with
   | Has.here, b => some b
   | Has.inl _, Sum.inl a => Has.out a
@@ -70,90 +93,124 @@ def Has.out {α β} [Spec α] [Spec β] [r: Has α β] : β → Option α
   | Has.inr _, Sum.inl _ => none
   | Has.inr _, Sum.inr a => Has.out a
 
-def Step (T : Type u) [Spec T] : IxPoly.Endo (Type v) where
-  Tag := fun α => NodeTag T α
-  Field := fun _=> NodeTag.fields
-  Elem := fun _ => NodeTag.elem
+def Step (Γ : Type u) (T : Γ → Type u) [Spec T] :
+    IxPoly.Endo (Γ × Type v) where
+  Tag := fun (γ, α) => NodeTag Γ T γ α
+  Field := fun _ n => n.fields
+  Elem := fun _ n p => n.elem p
 
-structure Tau : Type u
-instance : Spec Tau where
-  input := fun _ => PUnit
-  output := fun _ => PUnit
-  blockTag := fun _ => PEmpty
-  blockInputs := fun _ => nofun
-  blockOutputs := fun _ => nofun
+structure TauCarrier : Type v
+def Tau {Γ : Type u} : Γ → Type v := fun _ => TauCarrier
 
-structure Fail : Type u
-instance : Spec Fail where
-  input := fun _ => PUnit
-  output := fun _ => PEmpty
-  blockTag := fun _ => PEmpty
-  blockInputs := fun _ => nofun
-  blockOutputs := fun _ => nofun
+instance tauSpec {Γ : Type u} : Spec (Tau (Γ := Γ)) where
+  input := fun _ _ => PUnit
+  output := fun _ _ => PUnit
+  blockTag := fun _ _ => PEmpty
+  blockCtx := nofun
+  blockInputs := nofun
+  blockOutputs := nofun
+
+structure FailCarrier : Type v
+def Fail {Γ : Type u} : Γ → Type v := fun _ => FailCarrier
+
+instance failSpec {Γ : Type u} : Spec (Fail (Γ := Γ)) where
+  input := fun _ _ => PUnit
+  output := fun _ _ => PEmpty
+  blockTag := fun _ _ => PEmpty
+  blockCtx := nofun
+  blockInputs := nofun
+  blockOutputs := nofun
 
 namespace Step
 
-def ret {E α Y} [Spec E] (x : α) : Step E Y α := ⟨.ret x, fun a => PEmpty.elim a⟩
-def op {E α Y} [s: Spec E] (e : E) (inp : s.input e)
-    (blocks : (t : s.blockTag e) → s.blockInputs e t → Y (s.blockOutputs e t))
-    (k : (o : s.output e) → Y α) : Step E Y α :=
+def ret {Γ E α Y} {γ : Γ} [Spec E] (x : α) : Step Γ E Y (γ, α) := ⟨.ret x, fun a => PEmpty.elim a⟩
+def op {Γ E α Y} {γ : Γ} [s: Spec E] (e : E γ) (inp : s.input γ e)
+    (blocks : (t : s.blockTag γ e) → s.blockInputs γ e t → Y (s.blockCtx γ e t, s.blockOutputs γ e t))
+    (k : (o : s.output γ e) → Y (γ, α)) : Step Γ E Y (γ, α) :=
   ⟨.op e inp, fun
     | Sum.inl o => k o
     | Sum.inr ⟨t, i⟩ => blocks t i
   ⟩
 
-def Has.liftInput {E F} [s: Spec E] [s' : Spec F] (h : Has F E) (e : F) (inp : s'.input e) : s.input (Has.mk e) :=
+def Has.liftInput
+    {Γ : Type u} {E F : Γ → Type u} {γ : Γ}
+    [s : Spec E] [s' : Spec F]
+    (h : Has F E) (e : F γ) (inp : s'.input γ e) :
+    s.input γ (Has.mk (r := h) e) :=
   match h with
   | Has.here => inp
   | Has.inl r => liftInput r e inp
   | Has.inr r => liftInput r e inp
 
-def Has.lowerBlockTag {E F} [s: Spec E] [s' : Spec F] [h : Has F E] {e : F} (t : s.blockTag (Has.mk e)) : s'.blockTag e :=
+def Has.lowerBlockTag
+    {Γ : Type u} {E F : Γ → Type u} {γ : Γ}
+    [s : Spec E] [s' : Spec F] [h : Has F E]
+    {e : F γ} (t : s.blockTag γ (Has.mk (r := h) e)) :
+    s'.blockTag γ e :=
   match h with
   | Has.here => t
   | Has.inl r => lowerBlockTag (h:=r) t
   | Has.inr r => lowerBlockTag (h:=r) t
 
-def Has.lowerBlockInput {E F} [s: Spec E] [s' : Spec F] [h : Has F E]: {e : F} → (t : s.blockTag (Has.mk e)) →
-    (i : s.blockInputs (Has.mk e) t) → s'.blockInputs e (lowerBlockTag t) :=
+def Has.lowerBlockInput
+    {Γ : Type u} {E F : Γ → Type u} {γ : Γ}
+    [s : Spec E] [s' : Spec F] [h : Has F E] :
+    {e : F γ} →
+    (t : s.blockTag γ (Has.mk (r := h) e)) →
+    s.blockInputs γ (Has.mk (r := h) e) t →
+    s'.blockInputs γ e (lowerBlockTag t) :=
   match h with
   | Has.here => fun _ i => i
   | Has.inl r => fun t i => lowerBlockInput (h:=r) t i
   | Has.inr r => fun t i => lowerBlockInput (h:=r) t i
 
 def Has.liftBlockOutput
-    {E F} {Y : Type v → Type w}
+    {Γ : Type u} {E F : Γ → Type u} {γ : Γ}
+    {Y : Γ × Type v → Type w}
     [s : Spec E] [s' : Spec F] [h : Has F E] :
-    {e : F} →
-    (t : s.blockTag (Has.mk e)) →
-    Y (s'.blockOutputs e (Has.lowerBlockTag t)) →
-    Y (s.blockOutputs (Has.mk e) t) := match h with
+    {e : F γ} →
+    (t : s.blockTag γ (Has.mk (r := h) e)) →
+    Y (s'.blockCtx γ e (Has.lowerBlockTag t),
+      s'.blockOutputs γ e (Has.lowerBlockTag t)) →
+    Y (s.blockCtx γ (Has.mk (r := h) e) t,
+      s.blockOutputs γ (Has.mk (r := h) e) t) := match h with
   | Has.here => fun _ x => x
   | Has.inl r => fun t x => liftBlockOutput (h:=r) t x
   | Has.inr r => fun t x => liftBlockOutput (h:=r) t x
 
 def Has.lowerOutput
-    {E F} [s : Spec E] [s' : Spec F] [h : Has F E]
-    {e : F} (o : s.output (Has.mk e)) :
-    s'.output e := match h with
+    {Γ : Type u} {E F : Γ → Type u} {γ : Γ}
+    [s : Spec E] [s' : Spec F] [h : Has F E]
+    {e : F γ} (o : s.output γ (Has.mk (r := h) e)) :
+    s'.output γ e := match h with
   | Has.here => o
   | Has.inl r => lowerOutput (h:=r) o
   | Has.inr r => lowerOutput (h:=r) o
 
-def Has.op {E F α Y} [s: Spec E] [s': Spec F] [h: Has F E] (e : F) (inp : s'.input e)
-    (blocks : (t : s'.blockTag e) → s'.blockInputs e t → Y (s'.blockOutputs e t))
-    (k : (o : s'.output e) → Y α) : Step E Y α :=
+def Has.op
+    {Γ : Type u} {E F : Γ → Type u} {γ : Γ} {α : Type v}
+    {Y : Γ × Type v → Type w}
+    [s : Spec E] [s' : Spec F] [h : Has F E]
+    (e : F γ) (inp : s'.input γ e)
+    (blocks :
+      (t : s'.blockTag γ e) →
+      s'.blockInputs γ e t →
+      Y (s'.blockCtx γ e t, s'.blockOutputs γ e t))
+    (k : s'.output γ e → Y (γ, α)) :
+    Step Γ E Y (γ, α) :=
   Step.op (Has.mk e)
      (Has.liftInput h e inp)
      (fun t i => Has.liftBlockOutput t $ blocks (Has.lowerBlockTag t) (Has.lowerBlockInput t i))
      (fun o => k (Has.lowerOutput o))
 
- theorem Has.liftBlockOutput_naturality
-      {E F} {Y : Type v → Type w} {Z : Type v → Type z}
+theorem Has.liftBlockOutput_naturality
+      {Γ : Type u} {E F : Γ → Type u} {γ : Γ}
+      {Y : Γ × Type v → Type w} {Z : Γ × Type v → Type z}
       [s : Spec E] [s' : Spec F] [h : Has F E]
-      (f : (α : Type v) → Y α → Z α) {e : F}
-      (t : s.blockTag (Has.mk e))
-      (x : Y (s'.blockOutputs e (Has.lowerBlockTag t))) :
+      (f : (i : Γ × Type v) → Y i → Z i) {e : F γ}
+      (t : s.blockTag γ (Has.mk (r := h) e))
+      (x : Y (s'.blockCtx γ e (Has.lowerBlockTag t),
+        s'.blockOutputs γ e (Has.lowerBlockTag t))) :
       f _ (Has.liftBlockOutput (Y := Y) t x) =
         Has.liftBlockOutput (Y := Z) t (f _ x) := by
     induction h with
@@ -161,14 +218,31 @@ def Has.op {E F α Y} [s: Spec E] [s': Spec F] [h: Has F E] (e : F) (inp : s'.in
     | inl r ih => exact ih t x
     | inr r ih => exact ih t x
 
-def tau {E α Y} [Spec E] [Has Tau E] (x : Y α) : Step E Y α := Has.op Tau.mk () nofun (fun () => x)
+def tau
+    {Γ : Type u} {E : Γ → Type u} {γ : Γ} {α : Type v}
+    {Y : Γ × Type v → Type w}
+    [Spec E] [Has Tau E]
+    (x : Y (γ, α)) :
+    Step Γ E Y (γ, α) :=
+  Has.op (F := Tau) TauCarrier.mk PUnit.unit nofun
+    (fun _ => x)
 
-def fail {E α Y} [Spec E] [Has Fail E] : Step E Y α := Has.op Fail.mk () nofun nofun
+def fail
+    {Γ : Type u} {E : Γ → Type u} {γ : Γ} {α : Type v}
+    {Y : Γ × Type v → Type w}
+    [Spec E] [Has Fail E] :
+    Step Γ E Y (γ, α) :=
+  Has.op (F := Fail) FailCarrier.mk PUnit.unit nofun nofun
 
-protected def casesOn {E Y} [Spec E] { motive : (α : Type _) → Step E Y α → Sort* } {α} (x : Step E Y α)
-    (ret : ∀ {α} x, motive α (ret x))
-    (op : ∀ {α} e inp blocks k, motive α (op e inp blocks k)):
-    motive α x := by
+protected def casesOn
+    {Γ : Type u} {E : Γ → Type u}
+    {Y : Γ × Type v → Type w} [Spec E]
+    {motive : (i : Γ × Type v) → Step Γ E Y i → Sort z}
+    {i : Γ × Type v} (x : Step Γ E Y i)
+    (ret : ∀ {γ : Γ} {α : Type v} x, motive (γ, α) (ret x))
+    (op : ∀ {γ : Γ} {α : Type v} e inp blocks k,
+      motive (γ, α) (op e inp blocks k)) :
+    motive i x := by
   rcases x with ⟨tag, fields⟩
   cases tag with
   | ret a =>
@@ -183,8 +257,12 @@ protected def casesOn {E Y} [Spec E] { motive : (α : Type _) → Step E Y α �
     ext a; cases a <;> rfl
 
 @[simp]
-theorem map_ret {E} [Spec E] {Y Z : Type _ → Type _} {f : (α : Type _) → Y α → Z α} {α : Type _} {x : α}:
-    IxPoly.map (F := Step E) f α (Step.ret x) = Step.ret x := by
+theorem map_ret
+    {Γ : Type u} {E : Γ → Type u} [Spec E]
+    {Y : Γ × Type v → Type w} {Z : Γ × Type v → Type z}
+    {f : (i : Γ × Type v) → Y i → Z i}
+    {γ : Γ} {α : Type v} {x : α} :
+    IxPoly.map (F := Step Γ E) f (γ, α) (Step.ret x) = Step.ret x := by
   simp only [IxPoly.map, ret]
   congr 1
   ext a; cases a
@@ -199,28 +277,37 @@ theorem map_ret {E} [Spec E] {Y Z : Type _ → Type _} {f : (α : Type _) → Y 
 --   ext a; cases a
 
 @[simp]
-theorem map_op {E} [h: Spec E] {Y Z : Type _ → Type _} {f : (α : Type _) → Y α → Z α} {α : Type _}
-    {e : E} {inp : h.input e}
-    {blocks : (t : h.blockTag e) → h.blockInputs e t → Y (h.blockOutputs e t)}
-    {k : (o : h.output e) → Y α}:
-    IxPoly.map (F := Step E) f α (Step.op e inp blocks k) =
+theorem map_op
+    {Γ : Type u} {E : Γ → Type u} [h : Spec E]
+    {Y : Γ × Type v → Type w} {Z : Γ × Type v → Type z}
+    {f : (i : Γ × Type v) → Y i → Z i}
+    {γ : Γ} {α : Type v}
+    {e : E γ} {inp : h.input γ e}
+    {blocks :
+      (t : h.blockTag γ e) →
+      h.blockInputs γ e t →
+      Y (h.blockCtx γ e t, h.blockOutputs γ e t)}
+    {k : h.output γ e → Y (γ, α)} :
+    IxPoly.map (F := Step Γ E) f (γ, α) (Step.op e inp blocks k) =
       Step.op e inp (fun t i => f _ (blocks t i)) (fun o => f _ (k o)) := by
   simp only [IxPoly.map, op]
   congr 1
   ext a; cases a <;> rfl
 
-  @[simp]
-  theorem map_hasOp
-      {E F} [Spec E] [Spec F] [Has F E]
-      {Y Z : Type _ → Type _}
-      (f : (α : Type _) → Y α → Z α) {α}
-      (e : F) (inp : Spec.input e)
+@[simp]
+theorem map_hasOp
+      {Γ : Type u} {E F : Γ → Type u}
+      [Spec E] [Spec F] [Has F E]
+      {Y : Γ × Type v → Type w} {Z : Γ × Type v → Type z}
+      (f : (i : Γ × Type v) → Y i → Z i)
+      {γ : Γ} {α : Type v}
+      (e : F γ) (inp : Spec.input γ e)
       (blocks :
-        (t : Spec.blockTag e) →
-        Spec.blockInputs e t →
-        Y (Spec.blockOutputs e t))
-      (k : Spec.output e → Y α) :
-      IxPoly.map (F := Step E) f α (Has.op e inp blocks k) =
+        (t : Spec.blockTag γ e) →
+        Spec.blockInputs γ e t →
+        Y (Spec.blockCtx γ e t, Spec.blockOutputs γ e t))
+      (k : Spec.output γ e → Y (γ, α)) :
+      IxPoly.map (F := Step Γ E) f (γ, α) (Has.op e inp blocks k) =
         Has.op e inp
           (fun t i => f _ (blocks t i))
           (fun o => f _ (k o)) := by
@@ -231,8 +318,14 @@ theorem map_op {E} [h: Spec E] {Y Z : Type _ → Type _} {f : (α : Type _) → 
     apply Has.liftBlockOutput_naturality
 
 @[simp]
-theorem map_tau {E} [Spec E] [Has Tau E] {Y Z : Type _ → Type _} {f : (α : Type _) → Y α → Z α} {α : Type _} {x : Y α}:
-    IxPoly.map (F := Step E) f α (Step.tau x) = Step.tau (f α x) := by
+theorem map_tau
+    {Γ : Type u} {E : Γ → Type u}
+    [Spec E] [Has Tau E]
+    {Y : Γ × Type v → Type w} {Z : Γ × Type v → Type z}
+    {f : (i : Γ × Type v) → Y i → Z i}
+    {γ : Γ} {α : Type v} {x : Y (γ, α)} :
+    IxPoly.map (F := Step Γ E) f (γ, α) (Step.tau x) =
+      Step.tau (f (γ, α) x) := by
   simp only [tau, map_hasOp]
   congr 1
   ext a
