Freigen/Free.lean
@@ -4,71 +4,110 @@ import Freigen.Eff
 
 namespace Freigen
 
-variable {E : Type u} [eS: Eff.Spec E] {α β : Type}
+variable {Γ : Type u} {E : Γ → Type u} [eS : Eff.Spec.{u, v} E]
+  {γ : Γ} {α β : Type v}
 
-private def wBind {α β} (a : IxPoly.W (Eff.Step E) α) (f : α → IxPoly.W (Eff.Step E) β): IxPoly.W (Eff.Step E) β := match a with
-  | IxPoly.W.mk i p g => match p with
+private def wBind
+    {i : Γ × Type v}
+    (a : IxPoly.W (Eff.Step Γ E) i)
+    (f : i.2 → IxPoly.W (Eff.Step Γ E) (i.1, β)) :
+    IxPoly.W (Eff.Step Γ E) (i.1, β) :=
+  match a with
+  | IxPoly.W.mk _ p g =>
+    match p with
     | .ret a => f a
-    | .op e inp => IxPoly.W.mk (F := Eff.Step E) _ (Eff.NodeTag.op e inp) (fun
-      | .inl a => wBind (g (.inl a)) f
-      | .inr b => g (.inr b)
-    )
+    | .op e inp =>
+      IxPoly.W.mk (F := Eff.Step Γ E) _ (Eff.NodeTag.op e inp) fun
+        | .inl a =>
+          wBind (i := (i.1, i.2))
+            (show IxPoly.W (Eff.Step Γ E) (i.1, i.2) from g (.inl a)) f
+        | .inr b => g (.inr b)
 
-instance : Monad (IxPoly.W (Eff.Step E)) where
+private theorem wBind_pure
+    {i : Γ × Type v}
+    (x : IxPoly.W (Eff.Step Γ E) i) :
+    wBind (β := i.2) x
+      (fun a => IxPoly.W.roll (Eff.Step.ret (γ := i.1) a)) = x := by
+  induction x with
+  | mk i p g ih =>
+    cases p
+    · simp [wBind, IxPoly.W.roll, Eff.Step.ret]
+      ext a
+      cases a
+    · simp only [wBind]
+      congr 2
+      ext x
+      cases x
+      · simp only
+        apply_assumption
+      · rfl
+
+private theorem wBind_assoc
+    {i : Γ × Type v} {δ : Type v}
+    (a : IxPoly.W (Eff.Step Γ E) i)
+    (f : i.2 → IxPoly.W (Eff.Step Γ E) (i.1, β))
+    (g : β → IxPoly.W (Eff.Step Γ E) (i.1, δ)) :
+    wBind (wBind a f) g =
+      wBind a (fun x => wBind (i := (i.1, β)) (f x) g) := by
+  induction a with
+  | mk i p children ih =>
+    cases p
+    · rfl
+    · simp only [wBind]
+      rw [wBind]
+      congr 2
+      ext x
+      cases x
+      · simp only
+        apply ih
+      · rfl
+
+instance : Monad (fun α : Type v => IxPoly.W (Eff.Step Γ E) (γ, α)) where
   pure a := IxPoly.W.roll (Eff.Step.ret a)
   bind x f := wBind x f
 
-instance : LawfulMonad (IxPoly.W (Eff.Step E)) := LawfulMonad.mk' _
-  (by
-    intro _ x
-    change wBind x (fun a => IxPoly.W.roll (Eff.Step.ret a)) = x
-    induction x with
-    | mk i p g ih =>
-      cases p
-      · simp [wBind, IxPoly.W.roll, Eff.Step.ret]
-        ext a
-        cases a
-      · simp only [wBind]
-        congr
-        ext x
-        cases x
-        · simp only
-          apply_assumption
-        · rfl
-  )
-  (by intros; rfl)
-  (by
-    intro _ _ _ a f g
-    induction a with
-    | mk i p g ih =>
-      cases p
-      · rfl
-      · simp only [Bind.bind, wBind]
-        congr
-        ext x; cases x
-        · simp only
-          apply ih
-        · rfl
-  )
+instance : LawfulMonad (fun α : Type v => IxPoly.W (Eff.Step Γ E) (γ, α)) :=
+  LawfulMonad.mk' _
+    (by intros; apply wBind_pure)
+    (by intros; change wBind _ _ = _; rfl)
+    (by intros; apply wBind_assoc)
 
-def Free (E : Type u) [Eff.Spec E] (α : Type) : Type _ :=
-    ExactCodensity (IxPoly.W (Eff.Step E)) α
+def Free
+    {Γ : Type u} (E : Γ → Type u) [Eff.Spec.{u, v} E]
+    (γ : Γ) (α : Type v) : Type _ :=
+  ExactCodensity (fun α : Type v => IxPoly.W (Eff.Step Γ E) (γ, α)) α
 
-private def wOp (e : E) (inp : eS.input e)
-    (blocks : (t : eS.blockTag e) → eS.blockInputs e t → IxPoly.W (Eff.Step E) (eS.blockOutputs e t)):
-    IxPoly.W (Eff.Step E) (eS.output e) :=
-  IxPoly.W.mk (F := Eff.Step E) _ (Eff.NodeTag.op e inp) fun
-    | .inl a => pure a
+private def wOp
+    (e : E γ) (inp : eS.input γ e)
+    (blocks :
+      (t : eS.blockTag γ e) →
+      eS.blockInputs γ e t →
+      IxPoly.W (Eff.Step Γ E)
+        (eS.blockCtx γ e t, eS.blockOutputs γ e t)) :
+    IxPoly.W (Eff.Step Γ E) (γ, eS.output γ e) :=
+  IxPoly.W.mk (F := Eff.Step Γ E) _ (Eff.NodeTag.op e inp) fun
+    | .inl a =>
+      IxPoly.W.roll (F := Eff.Step Γ E) (Eff.Step.ret (γ := γ) a)
     | .inr ⟨b, i⟩ => blocks b i
 
-def Free.op (e : E) (inp : eS.input e)
-    (blocks : (t : eS.blockTag e) → eS.blockInputs e t → Free E (eS.blockOutputs e t)):
-    Free E (eS.output e) :=
-  ExactCodensity.equiv.symm $ wOp e inp (fun t i => ExactCodensity.equiv (blocks t i))
+def Free.op
+    (e : E γ) (inp : eS.input γ e)
+    (blocks :
+      (t : eS.blockTag γ e) →
+      eS.blockInputs γ e t →
+      Free E (eS.blockCtx γ e t) (eS.blockOutputs γ e t)) :
+    Free E γ (eS.output γ e) :=
+  ExactCodensity.equiv.symm <|
+    wOp e inp (fun t i => ExactCodensity.equiv (blocks t i))
 
-instance : Monad (Free E) :=
-  inferInstanceAs (Monad (ExactCodensity (IxPoly.W (Eff.Step E))))
-instance : LawfulMonad (Free E) :=
-  inferInstanceAs (LawfulMonad (ExactCodensity (IxPoly.W (Eff.Step E))))
+instance : Monad (Free E γ) :=
+  inferInstanceAs
+    (Monad (ExactCodensity
+      (fun α : Type v => IxPoly.W (Eff.Step Γ E) (γ, α))))
+
+instance : LawfulMonad (Free E γ) :=
+  inferInstanceAs
+    (LawfulMonad (ExactCodensity
+      (fun α : Type v => IxPoly.W (Eff.Step Γ E) (γ, α))))
 
 end Freigen
