Freigen/ITree/Basic.lean
@@ -3,101 +3,165 @@ import Freigen.Eff
 
 namespace Freigen
 
-def ITree (E : Type u) [Eff.Spec E] (α : Type _): Type _ := (Eff.Step E).M α
+def ITree
+    {Γ : Type u} (E : Γ → Type u) [Eff.Spec E]
+    (γ : Γ) (α : Type v) : Type _ :=
+  (Eff.Step Γ E).M (γ, α)
+
 namespace ITree
 
 open IxPoly
 
-variable {E : Type u} [eS : Eff.Spec E]
+variable {Γ : Type u} {E : Γ → Type u} [eS : Eff.Spec E]
 
-def corec {A : Type _ → Type _} (f : (i : Type _) → A i → Eff.Step E A i): {i : Type _} → A i → ITree E i :=
+def corec
+    {A : Γ × Type v → Type w}
+    (f : (i : Γ × Type v) → A i → Eff.Step Γ E A i) :
+    {i : Γ × Type v} → A i → ITree E i.1 i.2 :=
   IxPoly.M.corec f
 
-def observe {α} : ITree E α ≃ Eff.Step E (ITree E) α := IxPoly.M.observe
+def observe {γ : Γ} {α : Type v} :
+    ITree E γ α ≃ Eff.Step Γ E (fun i => ITree E i.1 i.2) (γ, α) :=
+  IxPoly.M.observe
 
-def roll {α} : Eff.Step E (ITree E) α → ITree E α := IxPoly.M.observe.symm
+def roll {γ : Γ} {α : Type v} :
+    Eff.Step Γ E (fun i => ITree E i.1 i.2) (γ, α) → ITree E γ α :=
+  IxPoly.M.observe.symm
 
-theorem observe_roll {α} (x : Eff.Step E (ITree E) α): observe (roll x) = x := observe.apply_symm_apply _
+theorem observe_roll {γ : Γ} {α : Type v}
+    (x : Eff.Step Γ E (fun i => ITree E i.1 i.2) (γ, α)) :
+    observe (roll x) = x :=
+  observe.apply_symm_apply _
 
-theorem roll_observe {α} (x : ITree E α): roll (observe x) = x := observe.symm_apply_apply _
+theorem roll_observe {γ : Γ} {α : Type v} (x : ITree E γ α) :
+    roll (observe x) = x :=
+  observe.symm_apply_apply _
 
-theorem observe_corec {A : Type _ → Type _} (f : (i : Type _) → A i → Eff.Step E A i) {i : Type _} (a : A i):
-    observe (corec f a) = IxPoly.map (fun _ y => corec f y) i (f i a) := IxPoly.M.observe_corec
+theorem observe_corec
+    {A : Γ × Type v → Type w}
+    (f : (i : Γ × Type v) → A i → Eff.Step Γ E A i)
+    {i : Γ × Type v} (a : A i) :
+    observe (corec f a) =
+      IxPoly.map (fun _ y => corec f y) i (f i a) :=
+  IxPoly.M.observe_corec
 
-def ret {α} (x : α) : ITree E α := roll $ Eff.Step.ret x
-def op {α} (e : E) (inp : eS.input e)
-    (blocks : (t : eS.blockTag e) → eS.blockInputs e t → ITree E (eS.blockOutputs e t))
-    (k : (o : eS.output e) → ITree E α) : ITree E α :=
+def ret {γ : Γ} {α : Type v} (x : α) : ITree E γ α :=
+  roll <| Eff.Step.ret x
+
+def op {γ : Γ} {α : Type v} (e : E γ) (inp : eS.input γ e)
+    (blocks :
+      (t : eS.blockTag γ e) →
+      eS.blockInputs γ e t →
+      ITree E (eS.blockCtx γ e t) (eS.blockOutputs γ e t))
+    (k : eS.output γ e → ITree E γ α) :
+    ITree E γ α :=
   roll $ Eff.Step.op e inp blocks k
 
-theorem roll_ret {α} (x : α) : roll (E:=E) (Eff.Step.ret x) = ret x := rfl
+theorem roll_ret {γ : Γ} {α : Type v} (x : α) :
+    roll (E := E) (Eff.Step.ret (γ := γ) x) = ret (γ := γ) x :=
+  rfl
 
-theorem roll_op {α} (e : E) (inp : eS.input e)
-    (blocks : (t : eS.blockTag e) → eS.blockInputs e t → ITree E (eS.blockOutputs e t))
-    (k : (o : eS.output e) → ITree E α) :
-    roll (E:=E) (Eff.Step.op e inp blocks k) = op e inp blocks k := rfl
+theorem roll_op {γ : Γ} {α : Type v} (e : E γ) (inp : eS.input γ e)
+    (blocks :
+      (t : eS.blockTag γ e) →
+      eS.blockInputs γ e t →
+      ITree E (eS.blockCtx γ e t) (eS.blockOutputs γ e t))
+    (k : eS.output γ e → ITree E γ α) :
+    roll (E := E) (Eff.Step.op e inp blocks k) = op e inp blocks k :=
+  rfl
 
 @[simp]
-theorem observe_ret {α} (x : α) : observe (ret x (E:=E)) = Eff.Step.ret x := rfl
+theorem observe_ret {γ : Γ} {α : Type v} (x : α) :
+    observe (ret x (E := E) (γ := γ)) = Eff.Step.ret x :=
+  rfl
 
 @[simp]
-theorem observe_op {α} (e : E) (inp : eS.input e)
-    (blocks : (t : eS.blockTag e) → eS.blockInputs e t → ITree E (eS.blockOutputs e t))
-    (k : (o : eS.output e) → ITree E α) :
-    observe (op e inp blocks k (E:=E)) = Eff.Step.op e inp blocks k := rfl
+theorem observe_op {γ : Γ} {α : Type v} (e : E γ) (inp : eS.input γ e)
+    (blocks :
+      (t : eS.blockTag γ e) →
+      eS.blockInputs γ e t →
+      ITree E (eS.blockCtx γ e t) (eS.blockOutputs γ e t))
+    (k : eS.output γ e → ITree E γ α) :
+    observe (op e inp blocks k (E := E)) = Eff.Step.op e inp blocks k :=
+  rfl
 
-protected def casesOn { motive : (α : Type _) → ITree E α → Sort* } {α} (x : ITree E α)
-    (ret : ∀ {α} x, motive α (ret x))
-    (op : ∀ {α} e inp blocks k, motive α (op e inp blocks k)):
-    motive α x := by
+protected def casesOn
+    {motive : (i : Γ × Type v) → ITree E i.1 i.2 → Sort w}
+    {γ : Γ} {α : Type v} (x : ITree E γ α)
+    (ret : ∀ {γ : Γ} {α : Type v} x, motive (γ, α) (ret x))
+    (op : ∀ {γ : Γ} {α : Type v} e inp blocks k,
+      motive (γ, α) (op e inp blocks k)) :
+    motive (γ, α) x := by
   have : x = roll (observe x) := (observe.symm_apply_apply _).symm
   rw [this]
   cases observe x using Eff.Step.casesOn <;> apply_assumption
 
 inductive BisimRelF
-    (R : (α : Type _) → ITree E α → ITree E α → Prop):
-    (α : Type _) → Eff.Step E (ITree E) α → Eff.Step E (ITree E) α → Prop where
-| ret {α} (x : α): BisimRelF R α (Eff.Step.ret x) (Eff.Step.ret x)
-| op {α} (e : E) (inp : eS.input e)
-    (k1 k2 : (o : eS.output e) → ITree E α)
-    (blocks1 blocks2 : (t : eS.blockTag e) → eS.blockInputs e t → ITree E (eS.blockOutputs e t))
-    (h1 : ∀ o, R _ (k1 o) (k2 o))
-    (h2 : ∀ t i, R _ (blocks1 t i) (blocks2 t i)):
-  BisimRelF R α (Eff.Step.op e inp blocks1 k1) (Eff.Step.op e inp blocks2 k2)
+    (R : (i : Γ × Type v) → ITree E i.1 i.2 → ITree E i.1 i.2 → Prop) :
+    (i : Γ × Type v) →
+    Eff.Step Γ E (fun i => ITree E i.1 i.2) i →
+    Eff.Step Γ E (fun i => ITree E i.1 i.2) i → Prop where
+| ret {γ : Γ} {α : Type v} (x : α) :
+    BisimRelF R (γ, α) (Eff.Step.ret x) (Eff.Step.ret x)
+| op {γ : Γ} {α : Type v} (e : E γ) (inp : eS.input γ e)
+    (k1 k2 : eS.output γ e → ITree E γ α)
+    (blocks1 blocks2 :
+      (t : eS.blockTag γ e) →
+      eS.blockInputs γ e t →
+      ITree E (eS.blockCtx γ e t) (eS.blockOutputs γ e t))
+    (h1 : ∀ o, R (γ, α) (k1 o) (k2 o))
+    (h2 : ∀ t i,
+      R (eS.blockCtx γ e t, eS.blockOutputs γ e t)
+        (blocks1 t i) (blocks2 t i)) :
+    BisimRelF R (γ, α)
+      (Eff.Step.op e inp blocks1 k1)
+      (Eff.Step.op e inp blocks2 k2)
 
-theorem BisimRelF.toLiftR {R : (α : Type _) → ITree E α → ITree E α → Prop} : BisimRelF R ≤ IxPoly.M.LiftR (Eff.Step E) R := by
-  intro α x y hxy
+theorem BisimRelF.toLiftR
+    {R : (i : Γ × Type v) → ITree E i.1 i.2 → ITree E i.1 i.2 → Prop} :
+    BisimRelF R ≤ IxPoly.M.LiftR (Eff.Step Γ E) R := by
+  intro i x y hxy
   cases hxy <;> constructor
   case ret => intro a; cases a
-  -- case tau => intro _; assumption
   case op =>
     intro a
     cases a <;> apply_assumption
 
 theorem BisimRelF.refl {R}
-    (hrefl : ∀ {α} (x : ITree E α), R α x x)
-    {α} (x : Eff.Step E (ITree E) α): BisimRelF R α x x := by
+    (hrefl : ∀ {i : Γ × Type v} (x : ITree E i.1 i.2), R i x x)
+    {i : Γ × Type v}
+    (x : Eff.Step Γ E (fun i => ITree E i.1 i.2) i) :
+    BisimRelF R i x x := by
   cases x using Eff.Step.casesOn <;> constructor <;> intros <;> apply_assumption
 
 theorem BisimRelF.refl_upToEq {R}
-    {α} (x : Eff.Step E (ITree E) α): BisimRelF (M.IxRel.upToEq R) α x x := by
+    {i : Γ × Type v}
+    (x : Eff.Step Γ E (fun i => ITree E i.1 i.2) i) :
+    BisimRelF (M.IxRel.upToEq R) i x x := by
   apply BisimRelF.refl
   intros
   apply Or.inl
   rfl
 
-theorem bisim {α} (R : (α : Type _) → ITree E α → ITree E α → Prop)
-    (step : ∀{α x y}, R α x y → BisimRelF R α (observe x) (observe y))
-    {x y : ITree E α} (hxy : R _ x y) : x = y := by
+theorem bisim
+    {γ : Γ} {α : Type v}
+    (R : (i : Γ × Type v) → ITree E i.1 i.2 → ITree E i.1 i.2 → Prop)
+    (step : ∀ {i x y}, R i x y → BisimRelF R i (observe x) (observe y))
+    {x y : ITree E γ α} (hxy : R (γ, α) x y) :
+    x = y := by
   apply IxPoly.M.Bisim.coind (R := R)
-  · intro α x y hxy
+  · intro i x y hxy
     apply BisimRelF.toLiftR
     apply step hxy
   · assumption
 
-theorem bisim_up_to_eq {α} (R : (α : Type _) → ITree E α → ITree E α → Prop)
-    (step : ∀{α x y}, R α x y → BisimRelF (M.IxRel.upToEq R) α (observe x) (observe y))
-    {x y : ITree E α} (hxy : R _ x y) : x = y := by
+theorem bisim_up_to_eq
+    {γ : Γ} {α : Type v}
+    (R : (i : Γ × Type v) → ITree E i.1 i.2 → ITree E i.1 i.2 → Prop)
+    (step : ∀ {i x y}, R i x y →
+      BisimRelF (M.IxRel.upToEq R) i (observe x) (observe y))
+    {x y : ITree E γ α} (hxy : R (γ, α) x y) :
+    x = y := by
   apply bisim (R := M.IxRel.upToEq R)
   · intro _ x y hxy
     cases hxy
@@ -109,29 +173,41 @@ theorem bisim_up_to_eq {α} (R : (α : Type _) → ITree E α → ITree E α →
   · right
     assumption
 
-theorem bisim₂ {α} {Seed : Type _ → Type _}
-    (left right : (i : Type _) → Seed i → ITree E i)
-    (step : ∀ {i} (s : Seed i), BisimRelF (M.IxRel.span Seed left right) i (observe (left i s)) (observe (right i s)))
-    (seed : Seed α): left α seed = right α seed := by
+theorem bisim₂
+    {i : Γ × Type v} {Seed : Γ × Type v → Type w}
+    (left right : (i : Γ × Type v) → Seed i → ITree E i.1 i.2)
+    (step : ∀ {i} (s : Seed i),
+      BisimRelF (M.IxRel.span Seed left right) i
+        (observe (left i s)) (observe (right i s)))
+    (seed : Seed i) :
+    left i seed = right i seed := by
   apply bisim (R := M.IxRel.span Seed left right)
   intro i x y hxy
   rcases hxy with ⟨s, rfl, rfl⟩
   apply step
   exists seed
 
-theorem bisim₂_up_to_eq {α} {Seed : Type _ → Type _}
-    (left right : (i : Type _) → Seed i → ITree E i)
-    (step : ∀ {i} (s : Seed i), BisimRelF (M.IxRel.upToEq (M.IxRel.span Seed left right)) i (observe (left i s)) (observe (right i s)))
-    (seed : Seed α): left α seed = right α seed := by
+theorem bisim₂_up_to_eq
+    {i : Γ × Type v} {Seed : Γ × Type v → Type w}
+    (left right : (i : Γ × Type v) → Seed i → ITree E i.1 i.2)
+    (step : ∀ {i} (s : Seed i),
+      BisimRelF (M.IxRel.upToEq (M.IxRel.span Seed left right)) i
+        (observe (left i s)) (observe (right i s)))
+    (seed : Seed i) :
+    left i seed = right i seed := by
   apply bisim_up_to_eq (R := M.IxRel.span Seed left right)
   intro i x y hxy
   rcases hxy with ⟨s, rfl, rfl⟩
   apply step
   exists seed
 
-def BindCarrier α R := (ITree E α × (α → ITree E R)) ⊕ ITree E R
-def bindCo {α : Type} (R : Type) :
-    BindCarrier (E:=E) α R → Eff.Step E (BindCarrier (E:=E) α) R
+abbrev BindCarrier
+    (E : Γ → Type u) [Eff.Spec E]
+    (α : Type v) (i : Γ × Type v) : Type _ :=
+  (ITree E i.1 α × (α → ITree E i.1 i.2)) ⊕ ITree E i.1 i.2
+
+def bindCo {α : Type v} (i : Γ × Type v) :
+    BindCarrier E α i → Eff.Step Γ E (BindCarrier E α) i
 | .inl (e, f) => match e.observe with
   | ⟨.ret x, _⟩ => IxPoly.map (fun _ => .inr) _ (f x).observe
   | ⟨.op e x, cont⟩ => ⟨.op e x, fun
@@ -140,75 +216,117 @@ def bindCo {α : Type} (R : Type) :
   ⟩
 | .inr e => IxPoly.map (fun _ => .inr) _ e.observe
 
-theorem bindCo_copy {α β : Type} {x : ITree E β} :
+theorem bindCo_copy
+    {α : Type v} {i : Γ × Type v} {x : ITree E i.1 i.2} :
     corec (bindCo (α := α)) (.inr x) = x := by
+  rcases i with ⟨γ, β⟩
   apply bisim (R := fun _ x y => x = corec (bindCo (α := α)) (.inr y))
-  intro _ x y hxy
+  intro j x y hxy
+  rcases j with ⟨δ, A⟩
   cases hxy
-  · simp only [observe_corec, bindCo, IxPoly.map_map]
-    cases y.observe using Eff.Step.casesOn <;> {
-       try simp; constructor <;> { intros ; apply_assumption }
-    }
+  · rw [observe_corec]
+    simp only [bindCo, IxPoly.map_map]
+    cases y.observe using Eff.Step.casesOn with
+    | ret =>
+      simp only [Eff.Step.map_ret]
+      constructor
+    | op =>
+      simp only [Eff.Step.map_op]
+      constructor <;> intros <;> rfl
   · rfl
 
-instance : Monad (ITree E) where
+instance {γ : Γ} : Monad (ITree E γ) where
   pure := fun x => ret x
-  bind {α β} (a : ITree E α) (f : α → ITree E β) := corec bindCo (.inl (a, f))
+  bind {α β} (a : ITree E γ α) (f : α → ITree E γ β) :=
+    corec bindCo ((.inl (a, f)) : BindCarrier E α (γ, β))
 
 @[simp]
-theorem ret_bind {α β : Type} {x : α}
-    {f : α → ITree E β} : ret x >>= f = f x := by
+theorem ret_bind
+    {γ : Γ} {α β : Type v} {x : α}
+    {f : α → ITree E γ β} :
+    ret x >>= f = f x := by
   apply observe.injective
-  simp only [Bind.bind, observe_corec, bindCo, ret,
-    observe_roll, IxPoly.map_map, Eff.Step.ret, bindCo_copy, IxPoly.map_id]
+  change observe
+      (corec bindCo
+        ((.inl (ret x, f)) : BindCarrier E α (γ, β))) =
+    observe (f x)
+  rw [observe_corec]
+  simp only [bindCo, observe_ret, Eff.Step.ret, IxPoly.map]
+  rcases observe (f x) with ⟨p, g⟩
+  change
+    (⟨p, fun a => corec bindCo (.inr (g a))⟩ :
+      Eff.Step Γ E (fun i => ITree E i.1 i.2) (γ, β)) =
+    ⟨p, g⟩
+  congr 1
+  funext a
+  exact bindCo_copy
 
 @[simp]
-theorem op_bind {α β : Type} {e : E} {inp : eS.input e}
-    {blocks : (t : eS.blockTag e) → eS.blockInputs e t → ITree E (eS.blockOutputs e t)}
-    {k : (o : eS.output e) → ITree E α}
-    {f : α → ITree E β}:
+theorem op_bind
+    {γ : Γ} {α β : Type v}
+    {e : E γ} {inp : eS.input γ e}
+    {blocks :
+      (t : eS.blockTag γ e) →
+      eS.blockInputs γ e t →
+      ITree E (eS.blockCtx γ e t) (eS.blockOutputs γ e t)}
+    {k : eS.output γ e → ITree E γ α}
+    {f : α → ITree E γ β} :
     (op e inp blocks k) >>= f =
       op e inp
         blocks
         (fun o => k o >>= f) := by
   apply observe.injective
-  simp only [Bind.bind, observe_corec, bindCo, op, observe_roll, IxPoly.map]
+  change observe
+      (corec bindCo
+        ((.inl (op e inp blocks k, f)) : BindCarrier E α (γ, β))) =
+    observe (op e inp blocks (fun o => k o >>= f))
+  rw [observe_corec]
+  simp only [bindCo, observe_op, IxPoly.map]
   simp only [Eff.Step.op]
-  congr
+  congr 2
   ext a; cases a
   · rfl
   · simp [bindCo_copy]
 
 @[simp]
 theorem hasOp_bind
-    {F : Type u} {α β : Type}
+    {F : Γ → Type u} {γ : Γ} {α β : Type v}
     [Eff.Spec F] [Eff.Has F E]
-    {e : F} {inp : Eff.Spec.input e}
+    {e : F γ} {inp : Eff.Spec.input γ e}
     {blocks :
-      (t : Eff.Spec.blockTag e) →
-      Eff.Spec.blockInputs e t →
-      ITree E (Eff.Spec.blockOutputs e t)}
-    {k : Eff.Spec.output e → ITree E α}
-    {f : α → ITree E β} :
+      (t : Eff.Spec.blockTag γ e) →
+      Eff.Spec.blockInputs γ e t →
+      ITree E (Eff.Spec.blockCtx γ e t) (Eff.Spec.blockOutputs γ e t)}
+    {k : Eff.Spec.output γ e → ITree E γ α}
+    {f : α → ITree E γ β} :
     (roll (Eff.Step.Has.op e inp blocks k) >>= f) =
       roll
         (Eff.Step.Has.op e inp blocks
           (fun o => k o >>= f)) := by
   simp only [Eff.Step.Has.op, roll_op, op_bind]
 
-inductive BindPureRel:
-    (α : Type) → ITree E α → ITree E α → Prop where
-| root {α} (m : ITree E α) : BindPureRel α (m >>= pure) m
-| refl {α} (m : ITree E α) : BindPureRel α m m
+inductive BindPureRel (γ : Γ) :
+    (α : Type v) → ITree E γ α → ITree E γ α → Prop where
+| root {α} (m : ITree E γ α) : BindPureRel γ α (m >>= pure) m
+| refl {α} (m : ITree E γ α) : BindPureRel γ α m m
 
-theorem bind_pure {α : Type} (a : ITree E α) :
+theorem bind_pure {γ : Γ} {α : Type v} (a : ITree E γ α) :
     a >>= pure = a := by
-  apply bisim₂_up_to_eq (Seed := ITree E) (left := fun _ x => x >>= pure) (right := fun _ x => x)
-  intro _ m
-  cases m using ITree.casesOn with
-  | ret => simp [pure, BisimRelF.refl_upToEq]
+  apply bisim₂_up_to_eq
+    (i := (γ, α))
+    (Seed := fun i => ITree E i.1 i.2)
+    (left := fun _ x => x >>= pure)
+    (right := fun _ x => x)
+    (seed := a)
+  intro i m
+  rcases i with ⟨δ, A⟩
+  have hm : m = roll (observe m) := (observe.symm_apply_apply _).symm
+  rw [hm]
+  cases observe m using Eff.Step.casesOn with
+  | ret =>
+    simp [roll_ret, ret_bind, pure, BisimRelF.refl_upToEq]
   | op e inp blocks k =>
-    simp only [op_bind]
+    simp only [roll_op, op_bind, observe_op]
     apply BisimRelF.op
     · intro
       right
@@ -216,26 +334,38 @@ theorem bind_pure {α : Type} (a : ITree E α) :
       apply And.intro <;> rfl
     · intros; left; rfl
 
-theorem bind_assoc {α β γ : Type}
-    {a : ITree E α} {f : α → ITree E β} {g : β → ITree E γ}:
+theorem bind_assoc
+    {δ : Γ} {α β γ : Type v}
+    {a : ITree E δ α}
+    {f : α → ITree E δ β}
+    {g : β → ITree E δ γ} :
     (a >>= f) >>= g = a >>= fun x => f x >>= g := by
-  apply bisim₂_up_to_eq (Seed := fun γ => ITree E α × (α → ITree E β) × (β → ITree E γ))
+  apply bisim₂_up_to_eq
+    (i := (δ, γ))
+    (Seed := fun i =>
+      ITree E i.1 α ×
+      (α → ITree E i.1 β) ×
+      (β → ITree E i.1 i.2))
     (left := fun _ ⟨x, f, g⟩ => (x >>= f) >>= g)
     (right := fun _ ⟨x, f, g⟩ => x >>= fun y => f y >>= g)
     (seed := ⟨a, f, g⟩)
-  intro _ ⟨x, f, g⟩
+  intro i ⟨x, f, g⟩
+  rcases i with ⟨ε, A⟩
   simp only
-  cases x using ITree.casesOn with
-  | ret => simp [BisimRelF.refl_upToEq]
+  have hx : x = roll (observe x) := (observe.symm_apply_apply _).symm
+  rw [hx]
+  cases observe x using Eff.Step.casesOn with
+  | ret =>
+    simp [roll_ret, ret_bind, BisimRelF.refl_upToEq]
   | op e inp blocks k =>
-    simp only [op_bind]
+    simp only [roll_op, op_bind, observe_op]
     apply BisimRelF.op
     · intro o
       right
       exists ⟨k o, f, g⟩
     · intros; left; rfl
 
-instance : LawfulMonad (ITree E) := LawfulMonad.mk' _
+instance {γ : Γ} : LawfulMonad (ITree E γ) := LawfulMonad.mk' _
   bind_pure
   (fun _ _ => ret_bind)
   (fun _ _ _ => bind_assoc)
@@ -244,70 +374,127 @@ section Loops
 
 variable [Eff.Has Eff.Tau E]
 
-def tau {α} (x : ITree E α) : ITree E α := roll $ Eff.Step.tau x
+def tau {γ : Γ} {α : Type v} (x : ITree E γ α) : ITree E γ α :=
+  roll $ Eff.Step.tau x
 
 @[simp]
-theorem observe_tau {α} (x : ITree E α) : observe (tau x) = Eff.Step.tau x := rfl
+theorem observe_tau {γ : Γ} {α : Type v} (x : ITree E γ α) :
+    observe (tau x) = Eff.Step.tau x := rfl
 
 @[simp]
-theorem tau_bind {α β : Type} {x : ITree E α}
-    {f : α → ITree E β} : tau x >>= f = tau (x >>= f) := by
+theorem tau_bind
+    {γ : Γ} {α β : Type v} {x : ITree E γ α}
+    {f : α → ITree E γ β} :
+    tau x >>= f = tau (x >>= f) := by
   apply observe.injective
   simp only [tau, Eff.Step.tau, hasOp_bind]
 
-private def LoopCarrier (E : Type u) [Eff.Spec E] (α β γ : Type) : Type _ :=
-    (ITree E (α ⊕ β) × (β → ITree E γ)) ⊕ ITree E γ
+private abbrev LoopCarrier
+    (E : Γ → Type u) [Eff.Spec E]
+    (α β : Type v) (i : Γ × Type v) : Type _ :=
+  ((α → ITree E i.1 (α ⊕ β)) ×
+    ITree E i.1 (α ⊕ β) ×
+    (β → ITree E i.1 i.2)) ⊕
+  ITree E i.1 i.2
 
-private def loopCo {α β : Type}
-    (body : α → ITree E (α ⊕ β)) (γ : Type):
-  LoopCarrier E α β γ → Eff.Step E (LoopCarrier E α β) γ
-| .inl (m, f) => match m.observe with
+private def loopCo {α β : Type v} (i : Γ × Type v) :
+    LoopCarrier E α β i → Eff.Step Γ E (LoopCarrier E α β) i
+| .inl (body, m, f) => match m.observe with
   | ⟨.ret (.inr v), _⟩ => IxPoly.map (fun _ => .inr) _ (f v).observe
-  | ⟨.ret (.inl v), _⟩ => Eff.Step.tau (.inl (body v, f))
+  | ⟨.ret (.inl v), _⟩ => Eff.Step.tau (.inl (body, body v, f))
   | ⟨.op e inp, k⟩ => Eff.Step.op e inp
       (fun t i => .inr (k $ .inr ⟨t, i⟩))
-      (fun o => .inl (k $ .inl o, f))
+      (fun o => .inl (body, k (.inl o), f))
 | .inr m => IxPoly.map (fun _ => .inr) _ m.observe
 
-private theorem loopCo_copy {α β γ : Type}
-    {body : α → ITree E (α ⊕ β)} {x : ITree E γ} :
-    corec (loopCo body) (.inr x) = x := by
-  apply bisim (R := fun _ x y => x = corec (loopCo body) (.inr y))
-  intro _ x y hxy
+private theorem observe_loopCo
+    {α β : Type v} {i : Γ × Type v}
+    (x : LoopCarrier E α β i) :
+    observe (corec (loopCo (E := E) (α := α) (β := β)) x) =
+      IxPoly.map
+        (fun _ y => corec (loopCo (E := E) (α := α) (β := β)) y)
+      i (loopCo i x) :=
+  observe_corec _ _
+
+private theorem loopCo_op
+    {α β δ : Type v} {γ : Γ}
+    (body : α → ITree E γ (α ⊕ β))
+    (e : E γ) (inp : eS.input γ e)
+    (blocks :
+      (t : eS.blockTag γ e) →
+      eS.blockInputs γ e t →
+      ITree E (eS.blockCtx γ e t) (eS.blockOutputs γ e t))
+    (next : eS.output γ e → ITree E γ (α ⊕ β))
+    (k : β → ITree E γ δ) :
+    loopCo (γ, δ)
+        ((.inl (body, op e inp blocks next, k)) :
+          LoopCarrier E α β (γ, δ)) =
+      Eff.Step.op e inp
+        (fun t i => .inr (blocks t i))
+        (fun o => .inl (body, next o, k)) := by
+  simp only [loopCo, observe_op, Eff.Step.op]
+
+private theorem loopCo_copy
+    {α β : Type v} {i : Γ × Type v}
+    {x : ITree E i.1 i.2} :
+    corec (loopCo (α := α) (β := β)) (.inr x) = x := by
+  rcases i with ⟨γ, δ⟩
+  apply bisim
+    (R := fun i x y =>
+      x = corec (loopCo (α := α) (β := β)) (.inr y))
+  intro j x y hxy
+  rcases j with ⟨ε, A⟩
   cases hxy
-  · simp only [observe_corec, loopCo, IxPoly.map_map]
-    cases y.observe using Eff.Step.casesOn <;> {
-       try simp; constructor <;> { intros ; apply_assumption }
-    }
+  · rw [observe_corec]
+    simp only [loopCo, IxPoly.map_map]
+    cases y.observe using Eff.Step.casesOn with
+    | ret =>
+      simp only [Eff.Step.map_ret]
+      constructor
+    | op =>
+      simp only [Eff.Step.map_op]
+      constructor <;> intros <;> rfl
   · rfl
 
-def loop {α β γ : Type} (body : α → ITree E (α ⊕ β))
-    (initial : α) (k : β → ITree E γ) : ITree E γ :=
-  corec (loopCo body) (.inl (body initial, k))
+def loop
+    {γ : Γ} {α β δ : Type v}
+    (body : α → ITree E γ (α ⊕ β))
+    (initial : α) (k : β → ITree E γ δ) :
+    ITree E γ δ :=
+  corec loopCo
+    ((.inl (body, body initial, k)) : LoopCarrier E α β (γ, δ))
 
-theorem loop_def {α β γ : Type}
-    {body : α → ITree E (α ⊕ β)}
-    {initial : α} {k : β → ITree E γ} :
+theorem loop_def
+    {γ : Γ} {α β δ : Type v}
+    {body : α → ITree E γ (α ⊕ β)}
+    {initial : α} {k : β → ITree E γ δ} :
     loop body initial k =
       (body initial >>= fun x => match x with
         | .inr v => k v
         | .inl v => tau (loop body v k)) := by
   unfold loop
   apply bisim₂_up_to_eq
+    (i := (γ, δ))
     (Seed := LoopCarrier E α β)
-    (left := fun _ x => corec (loopCo body) x)
+    (left := fun _ x => corec loopCo x)
     (right := fun _ x => match x with
       | .inr t => t
-      | .inl (m, f) => m >>= fun x => match x with
+      | .inl (body, m, f) => m >>= fun x => match x with
         | .inr v => f v
-        | .inl v => tau $ corec (loopCo body) (.inl (body v, f)))
-    (seed := .inl (body initial, k))
+        | .inl v => tau $ corec loopCo (.inl (body, body v, f)))
+    (seed :=
+      ((.inl (body, body initial, k)) :
+        LoopCarrier E α β (γ, δ)))
   intro i x
+  rcases i with ⟨ε, A⟩
   cases x with
   | inr m =>
-    simp only [observe_corec, loopCo, IxPoly.map_map]
+    rw [observe_corec]
+    simp only [loopCo, IxPoly.map_map]
     cases m.observe using Eff.Step.casesOn with
-    | ret => simp [BisimRelF.refl_upToEq]
+    | ret =>
+      simp only [Eff.Step.map_ret]
+      apply BisimRelF.refl_upToEq
     | op e inp blocks k =>
       simp only [Eff.Step.map_op]
       apply BisimRelF.op
@@ -318,19 +505,31 @@ theorem loop_def {α β γ : Type}
         left
         exact loopCo_copy
   | inl m =>
-    rcases m with ⟨m, f⟩
+    rcases m with ⟨body, m, f⟩
     simp only
-    have : m = roll (observe m) := (observe.symm_apply_apply _).symm
-    rw [this]
-    cases m.observe using Eff.Step.casesOn with
+    have hm : m = roll (observe m) := (observe.symm_apply_apply _).symm
+    rw [hm]
+    cases observe m using Eff.Step.casesOn with
     | ret x =>
       simp only [roll_ret, ret_bind]
       cases x with
       | inr v =>
-        simp only [observe_corec, loopCo, observe_ret, Eff.Step.ret, map_map, loopCo_copy, IxPoly.map_id]
+        simp only
+        rw [observe_loopCo
+          (E := E) (α := α) (β := β)
+          ((.inl (body, ret (.inr v), f)) :
+            LoopCarrier E α β (ε, A))]
+        simp only [loopCo, observe_ret, Eff.Step.ret, IxPoly.map_map,
+          loopCo_copy, IxPoly.map_id]
         apply BisimRelF.refl_upToEq
       | inl v =>
-        simp only [observe_tau, observe_corec, loopCo, observe_ret, Eff.Step.ret, Eff.Step.map_tau]
+        simp only
+        rw [observe_loopCo
+          (E := E) (α := α) (β := β)
+          ((.inl (body, ret (.inl v), f)) :
+            LoopCarrier E α β (ε, A))]
+        simp only [loopCo, observe_ret, Eff.Step.ret, Eff.Step.map_tau,
+          observe_tau]
         apply BisimRelF.op
         · intro
           left
@@ -338,77 +537,111 @@ theorem loop_def {α β γ : Type}
         · intro t
           exact (nomatch Eff.Step.Has.lowerBlockTag t)
     | op e inp blocks k =>
-      simp only [roll_op, observe_corec, loopCo, observe_op, op_bind]
-      conv => enter [3,3]; rw [Eff.Step.op]
-      simp only [Eff.Step.map_op]
+      simp only [roll_op, op_bind]
+      rw [observe_loopCo
+        (E := E) (α := α) (β := β)
+        ((.inl (body, op e inp blocks k, f)) :
+          LoopCarrier E α β (ε, A))]
+      rw [loopCo_op, Eff.Step.map_op]
+      simp only [observe_op]
       apply BisimRelF.op
       · intro o
         right
-        exists (.inl (k o, f))
+        exists (.inl (body, k o, f))
       · intros
         left
         exact loopCo_copy
 
-private theorem loopCo_bind {α β γ : Type}
-    (body : α → ITree E (α ⊕ β))
-    (m : ITree E (α ⊕ β)) (k : β → ITree E γ) :
-    corec (loopCo body) (.inl (m, pure)) >>= k =
-      corec (loopCo body) (.inl (m, k)) := by
+private theorem loopCo_bind
+    {γ : Γ} {α β δ : Type v}
+    (body : α → ITree E γ (α ⊕ β))
+    (m : ITree E γ (α ⊕ β)) (k : β → ITree E γ δ) :
+    (corec loopCo
+      ((.inl (body, m, pure)) : LoopCarrier E α β (γ, β)) >>= k) =
+      corec loopCo
+        ((.inl (body, m, k)) : LoopCarrier E α β (γ, δ)) := by
   symm
   apply bisim₂_up_to_eq
-    (Seed := fun γ => ITree E (α ⊕ β) × (β → ITree E γ))
-    (left := fun i ⟨m, k⟩ =>
-      corec (loopCo body) ((.inl (m, k)) : LoopCarrier (E:=E) α β i))
-    (right := fun _ ⟨m, k⟩ =>
-      corec (loopCo body) ((.inl (m, pure)) : LoopCarrier (E:=E) α β β) >>= k)
-    (seed := ⟨m, k⟩)
+    (i := (γ, δ))
+    (Seed := fun i =>
+      (α → ITree E i.1 (α ⊕ β)) ×
+      ITree E i.1 (α ⊕ β) ×
+      (β → ITree E i.1 i.2))
+    (left := fun _ ⟨body, m, k⟩ =>
+      corec loopCo (.inl (body, m, k)))
+    (right := fun i ⟨body, m, k⟩ =>
+      (corec loopCo
+        ((.inl (body, m, pure)) : LoopCarrier E α β (i.1, β)) :
+          ITree E i.1 β) >>= k)
+    (seed := ⟨body, m, k⟩)
   intro i seed
-  rcases seed with ⟨m, k⟩
+  rcases i with ⟨ε, A⟩
+  rcases seed with ⟨body, m, k⟩
   have hm : m = roll (observe m) := (observe.symm_apply_apply _).symm
   rw [hm]
   cases observe m using Eff.Step.casesOn with
   | ret x =>
     cases x with
     | inr v =>
-      have unfold : ∀ {j : Type} (f : β → ITree E j),
-          corec (loopCo body) (.inl (ret (.inr v), f)) = f v := by
+      have unfold : ∀ {j : Type v} (f : β → ITree E ε j),
+          corec loopCo
+            ((.inl (body, ret (.inr v), f)) :
+              LoopCarrier E α β (ε, j)) = f v := by
         intro j f
         apply observe.injective
-        simp only [observe_corec, loopCo, observe_ret, Eff.Step.ret, IxPoly.map_map,
+        rw [observe_loopCo]
+        simp only [loopCo, observe_ret, Eff.Step.ret, IxPoly.map_map,
           loopCo_copy, IxPoly.map_id]
       simp only [roll_ret]
       rw [unfold k, unfold pure]
       simp only [pure, ret_bind]
       apply BisimRelF.refl_upToEq
     | inl v =>
-      have unfold : ∀ {j : Type} (f : β → ITree E j),
-          corec (loopCo body) (.inl (ret (.inl v), f)) =
-            tau (corec (loopCo body) (.inl (body v, f))) := by
+      have unfold : ∀ {j : Type v} (f : β → ITree E ε j),
+          corec loopCo
+              ((.inl (body, ret (.inl v), f)) :
+                LoopCarrier E α β (ε, j)) =
+            tau
+              (corec loopCo
+                ((.inl (body, body v, f)) :
+                  LoopCarrier E α β (ε, j))) := by
         intro j f
         apply observe.injective
-        simp only [observe_corec, loopCo, observe_ret, Eff.Step.ret, Eff.Step.map_tau, observe_tau]
+        rw [observe_loopCo]
+        simp only [loopCo, observe_ret, Eff.Step.ret, Eff.Step.map_tau,
+          observe_tau]
+        rfl
       simp only [roll_ret]
       rw [unfold k, unfold pure]
       simp only [tau_bind, observe_tau]
       apply BisimRelF.op
       · intro
         right
-        exists ⟨body v, k⟩
+        exists ⟨body, body v, k⟩
       · intro t
         exact (nomatch Eff.Step.Has.lowerBlockTag t)
   | op e inp blocks next =>
-    have unfold : ∀ {j : Type} (f : β → ITree E j),
-        corec (loopCo body) (.inl (op e inp blocks next, f)) =
-          op e inp blocks (fun o => corec (loopCo body) (.inl (next o, f))) := by
+    have unfold : ∀ {j : Type v} (f : β → ITree E ε j),
+        corec loopCo
+            ((.inl (body, op e inp blocks next, f)) :
+              LoopCarrier E α β (ε, j)) =
+          op (E := E) (α := j) e inp blocks
+            (fun o =>
+              corec loopCo
+                ((.inl (body, next o, f)) :
+                  LoopCarrier E α β (ε, j))) := by
       intro j f
       apply observe.injective
       have hco :
-          loopCo body j (.inl (op e inp blocks next, f)) =
+          loopCo (ε, j) (.inl (body, op e inp blocks next, f)) =
             Eff.Step.op e inp
-              (fun t x => (.inr (blocks t x) : LoopCarrier (E:=E) α β (eS.blockOutputs e t)))
-              (fun o => .inl (next o, f)) := by
+              (fun t x =>
+                (.inr (blocks t x) :
+                  LoopCarrier E α β
+                    (eS.blockCtx ε e t, eS.blockOutputs ε e t)))
+              (fun o => .inl (body, next o, f)) := by
         simp only [loopCo, observe_op, Eff.Step.op]
-      rw [observe_corec, observe_op, hco, Eff.Step.map_op]
+      rw [observe_loopCo, observe_op, hco, Eff.Step.map_op]
       congr 1
       funext t x
       exact loopCo_copy
@@ -418,14 +651,15 @@ private theorem loopCo_bind {α β γ : Type}
     apply BisimRelF.op
     · intro o
       right
-      exists ⟨next o, k⟩
+      exists ⟨body, next o, k⟩
     · intros
       left
       rfl
 
-theorem loop_bind {α β γ : Type}
-    (body : α → ITree E (α ⊕ β))
-    (initial : α) (k : β → ITree E γ) :
+theorem loop_bind
+    {γ : Γ} {α β δ : Type v}
+    (body : α → ITree E γ (α ⊕ β))
+    (initial : α) (k : β → ITree E γ δ) :
     loop body initial pure >>= k = loop body initial k :=
   loopCo_bind body (body initial) k
 
@@ -434,10 +668,12 @@ end Loops
 section Fail
 
 variable [Eff.Has Eff.Fail E]
-def fail {α} : ITree E α := roll $ Eff.Step.fail
+def fail {γ : Γ} {α : Type v} : ITree E γ α := roll $ Eff.Step.fail
 
 @[simp]
-theorem fail_bind {α β : Type} {f : α → ITree E β} : fail >>= f = fail := by
+theorem fail_bind
+    {γ : Γ} {α β : Type v} {f : α → ITree E γ β} :
+    fail >>= f = fail := by
   apply observe.injective
   simp only [fail, Eff.Step.fail, hasOp_bind, observe_roll]
   congr
